ConNF/External/WellOrder.lean
@@ -23,9 +23,259 @@ variable [Params.{u}] {α β γ δ ε ζ : Λ} (hβ : (β : TypeIndex) < α) (h�
 /-- A set in our model that is a well-order. Internal well-orders are exactly external well-orders,
 so we externalise the definition for convenience. -/
 def InternalWellOrder (r : TSet α) : Prop :=
-  IsWellOrder (TSet δ) (ExternalRel hβ hγ hδ r)
+  IsWellOrder (ExternalRel hβ hγ hδ r).field
+    (InvImage (ExternalRel hβ hγ hδ r) Subtype.val)
 
 def InternallyWellOrdered (x : TSet γ) : Prop :=
-  ∃ r, InternalWellOrder hβ hγ hδ r ∧ x = dom hβ hγ hδ r
+  {y : TSet δ | y ∈' x}.Subsingleton ∨ (∃ r, InternalWellOrder hβ hγ hδ r ∧ x = field hβ hγ hδ r)
+
+@[simp]
+theorem externalRel_smul (r : TSet α) (ρ : AllPerm α) :
+    ExternalRel hβ hγ hδ (ρ • r) =
+      InvImage (ExternalRel hβ hγ hδ r) ((ρ ↘ hβ ↘ hγ ↘ hδ)⁻¹ • ·) := by
+  ext a b
+  simp only [ExternalRel, mem_smul_iff', allPerm_inv_sderiv', smul_op, InvImage]
+
+omit [Params] in
+/-- Well-orders are rigid. -/
+theorem apply_eq_of_isWellOrder {X : Type _} {r : Rel X X} {f : X → X}
+    (hr : IsWellOrder X r) (hf : Function.Bijective f) (hf' : ∀ x y, r x y ↔ r (f x) (f y)) :
+    ∀ x, f x = x := by
+  let emb : r ≼i r := ⟨⟨⟨f, hf.injective⟩, λ {a b} ↦ (hf' a b).symm⟩, ?_⟩
+  · have : emb = InitialSeg.refl r := Subsingleton.elim _ _
+    intro x
+    exact congr_arg (λ f ↦ f x) this
+  · intro a b h
+    exact hf.surjective _
+
+omit [Params] in
+theorem apply_eq_of_isWellOrder' {X : Type _} {r : Rel X X} {f : X → X}
+    (hr : IsWellOrder r.field (InvImage r Subtype.val)) (hf : Function.Bijective f)
+    (hf' : ∀ x y, r x y ↔ r (f x) (f y)) :
+    ∀ x ∈ r.field, f x = x := by
+  have : ∀ x ∈ r.field, f x ∈ r.field := by
+    rintro x (⟨y, h⟩ | ⟨y, h⟩)
+    · exact Or.inl ⟨f y, (hf' x y).mp h⟩
+    · exact Or.inr ⟨f y, (hf' y x).mp h⟩
+  have := apply_eq_of_isWellOrder (f := λ x ↦ ⟨f x.val, this x.val x.prop⟩) hr ⟨?_, ?_⟩ ?_
+  · intro x hx
+    exact congr_arg Subtype.val (this ⟨x, hx⟩)
+  · intro x y h
+    rw [Subtype.mk.injEq] at h
+    exact Subtype.val_injective (hf.injective h)
+  · intro x
+    obtain ⟨y, hy⟩ := hf.surjective x.val
+    refine ⟨⟨y, ?_⟩, ?_⟩
+    · obtain (⟨z, h⟩ | ⟨z, h⟩) := x.prop <;>
+          rw [← hy] at h <;>
+          obtain ⟨z, rfl⟩ := hf.surjective z
+      · exact Or.inl ⟨z, (hf' y z).mpr h⟩
+      · exact Or.inr ⟨z, (hf' z y).mpr h⟩
+    · simp only [hy]
+  · intros
+    apply hf'
+
+theorem exists_common_support_of_internallyWellOrdered' {x : TSet δ}
+    (h : InternallyWellOrdered hγ hδ hε x) :
+    ∃ S : Support β, ∀ y, y ∈' x → S.Supports { { {y}' }' }[hγ] := by
+  obtain (h | ⟨r, h, rfl⟩) := h
+  · obtain (h | ⟨y, hy⟩) := h.eq_empty_or_singleton
+    · use ⟨Enumeration.empty, Enumeration.empty⟩
+      intro y hy
+      rw [Set.eq_empty_iff_forall_not_mem] at h
+      cases h y hy
+    · obtain ⟨S, hS⟩ := TSet.exists_support y
+      use S ↗ hε ↗ hδ ↗ hγ
+      intro z hz
+      rw [Set.eq_singleton_iff_unique_mem] at hy
+      cases hy.2 z hz
+      refine ⟨?_, λ h ↦ by cases h⟩
+      intro ρ hρ
+      simp only [Support.smul_scoderiv, ← allPermSderiv_forget', Support.scoderiv_inj] at hρ
+      simp only [smul_singleton, singleton_inj]
+      exact hS _ hρ
+  obtain ⟨S, hS⟩ := TSet.exists_support r
+  use S
+  intro a ha
+  refine ⟨?_, λ h ↦ by cases h⟩
+  intro ρ hρ
+  have := hS ρ hρ
+  simp only [smul_singleton, singleton_inj]
+  apply apply_eq_of_isWellOrder' (r := ExternalRel hγ hδ hε r)
+  · exact h
+  · exact MulAction.bijective (ρ ↘ hγ ↘ hδ ↘ hε)
+  · intro x y
+    conv_rhs => rw [← this]
+    simp only [externalRel_smul, InvImage, inv_smul_smul]
+  · rwa [mem_field_iff] at ha
+
+include hγ in
+theorem Support.Supports.ofSingleton {S : Support α} {x : TSet β}
+    (h : S.Supports {x}') :
+    letI : Level := ⟨α⟩
+    letI : LeLevel α := ⟨le_rfl⟩
+    (S.strong ↘ hβ).Supports x := by
+  refine ⟨?_, λ h ↦ by cases h⟩
+  intro ρ hρ
+  open scoped Pointwise in
+  have := sUnion_singleton_symmetric_aux hγ hβ {y | y ∈' x} S ?_ ρ hρ
+  · apply ConNF.ext hγ
+    intro z
+    simp only [Set.ext_iff, Set.mem_setOf_eq, Set.mem_smul_set_iff_inv_smul_mem] at this
+    rw [mem_smul_iff', allPerm_inv_sderiv', this]
+  · intro ρ hρ
+    ext z
+    simp only [Set.mem_smul_set_iff_inv_smul_mem, Set.mem_image, Set.mem_setOf_eq]
+    have := h.supports ρ hρ
+    simp only [smul_singleton, singleton_inj] at this
+    constructor
+    · rintro ⟨y, h₁, h₂⟩
+      rw [← smul_eq_iff_eq_inv_smul, smul_singleton] at h₂
+      refine ⟨_, ?_, h₂⟩
+      rw [← this]
+      simp only [mem_smul_iff', allPerm_inv_sderiv', inv_smul_smul]
+      exact h₁
+    · rintro ⟨y, h, rfl⟩
+      refine ⟨(ρ ↘ hβ ↘ hγ)⁻¹ • y, ?_, ?_⟩
+      · rwa [← allPerm_inv_sderiv', ← mem_smul_iff', this]
+      · simp only [smul_singleton, allPerm_inv_sderiv']
+
+include hγ in
+theorem supports_of_supports_singletons {S : Support α} {s : Set (TSet β)}
+    (h : ∀ x ∈ s, S.Supports {x}') :
+    ∃ S : Support β, ∀ x ∈ s, S.Supports x :=
+  ⟨_, λ x hx ↦ (h x hx).ofSingleton hβ hγ⟩
+
+theorem exists_common_support_of_internallyWellOrdered {x : TSet δ}
+    (h : InternallyWellOrdered hγ hδ hε x) :
+    ∃ S : Support δ, ∀ y, y ∈' x → S.Supports {y}' := by
+  obtain ⟨S, hS⟩ := exists_common_support_of_internallyWellOrdered' hγ hδ hε h
+  have := supports_of_supports_singletons (S := S)
+      (s := singleton hδ '' (singleton hε '' {y | y ∈' x})) hγ hδ ?_
+  swap
+  · simp only [Set.mem_image, Set.mem_setOf_eq, exists_exists_and_eq_and, forall_exists_index,
+      and_imp, forall_apply_eq_imp_iff₂]
+    exact hS
+  obtain ⟨T, hT⟩ := this
+  have := supports_of_supports_singletons (S := T)
+      (s := singleton hε '' {y | y ∈' x}) hδ hε ?_
+  swap
+  · simp only [Set.mem_image, Set.mem_setOf_eq, forall_exists_index, and_imp,
+      forall_apply_eq_imp_iff₂] at hT ⊢
+    exact hT
+  simp only [Set.mem_image, Set.mem_setOf_eq, forall_exists_index, and_imp,
+    forall_apply_eq_imp_iff₂] at this
+  exact this
+
+theorem internallyWellOrdered_of_common_support_of_nontrivial {x : TSet γ}
+    (hx : {y : TSet δ | y ∈' x}.Nontrivial)
+    (S : Support δ) (hS : ∀ y : TSet δ, y ∈' x → S.Supports y) :
+    InternallyWellOrdered hβ hγ hδ x := by
+  have := exists_of_symmetric
+      {p : TSet β | ∃ a b : TSet δ, p = ⟨a, b⟩' ∧ a ∈' x ∧ b ∈' x ∧ WellOrderingRel a b} hβ ?_
+  swap
+  · use S ↗ hδ ↗ hγ ↗ hβ
+    intro ρ hρ
+    ext z
+    simp only [Support.smul_scoderiv, ← allPermSderiv_forget', Support.scoderiv_inj] at hρ
+    simp only [Set.mem_smul_set_iff_inv_smul_mem, Set.mem_setOf_eq]
+    constructor
+    · rintro ⟨a, b, h₁, h₂, h₃, h₄⟩
+      refine ⟨a, b, ?_, h₂, h₃, h₄⟩
+      rw [inv_smul_eq_iff] at h₁
+      rw [h₁, smul_op, op_inj]
+      exact ⟨(hS a h₂).supports _ hρ, (hS b h₃).supports _ hρ⟩
+    · rintro ⟨a, b, h₁, h₂, h₃, h₄⟩
+      refine ⟨a, b, ?_, h₂, h₃, h₄⟩
+      rw [h₁, smul_op, op_inj]
+      simp only [allPerm_inv_sderiv', inv_smul_eq_iff]
+      rw [(hS a h₂).supports _ hρ, (hS b h₃).supports _ hρ]
+      exact ⟨rfl, rfl⟩
+  obtain ⟨r, hr⟩ := this
+  right
+  use r
+  have hr' : ∀ a b, ExternalRel hβ hγ hδ r a b ↔ a ∈' x ∧ b ∈' x ∧ WellOrderingRel a b := by
+    intro a b
+    rw [ExternalRel, hr]
+    simp only [Set.mem_setOf_eq, op_inj]
+    constructor
+    · rintro ⟨a, b, ⟨rfl, rfl⟩, h⟩
+      exact h
+    · intro h
+      exact ⟨a, b, ⟨rfl, rfl⟩, h⟩
+  have hrx : ∀ a, a ∈ (ExternalRel hβ hγ hδ r).field ↔ a ∈' x := by
+    intro a
+    constructor
+    · rintro (⟨b, h⟩ | ⟨b, h⟩)
+      · rw [hr'] at h
+        exact h.1
+      · rw [hr'] at h
+        exact h.2.1
+    · intro h
+      obtain ⟨b, h₁, h₂⟩ := hx.exists_ne a
+      obtain (h₃ | h₃ | h₃) := WellOrderingRel.isWellOrder.trichotomous a b
+      · refine Or.inl ⟨b, ?_⟩
+        rw [hr']
+        exact ⟨h, h₁, h₃⟩
+      · cases h₂ h₃.symm
+      · refine Or.inr ⟨b, ?_⟩
+        rw [hr']
+        exact ⟨h₁, h, h₃⟩
+  refine ⟨?_, ?_⟩
+  swap
+  · apply ext hδ
+    intro z
+    rw [mem_field_iff, hrx]
+  refine @IsWellOrder.mk _ _ ?_ ?_ ?_
+  · constructor
+    intro a b
+    obtain (h | h | h) := WellOrderingRel.isWellOrder.trichotomous a.val b.val
+    · apply Or.inl
+      rw [InvImage, hr']
+      exact ⟨(hrx a).mp a.prop, (hrx b).mp b.prop, h⟩
+    · exact Or.inr (Or.inl (Subtype.val_injective h))
+    · apply Or.inr ∘ Or.inr
+      rw [InvImage, hr']
+      exact ⟨(hrx b).mp b.prop, (hrx a).mp a.prop, h⟩
+  · constructor
+    intro a b c h₁ h₂
+    rw [InvImage, hr'] at h₁ h₂ ⊢
+    exact ⟨h₁.1, h₂.2.1, WellOrderingRel.isWellOrder.trans _ _ _ h₁.2.2 h₂.2.2⟩
+  · constructor
+    apply InvImage.wf
+    refine Subrelation.wf ?_ WellOrderingRel.isWellOrder.wf
+    intro a b h
+    rw [hr'] at h
+    exact h.2.2
+
+theorem internallyWellOrdered_of_common_support {x : TSet γ}
+    (S : Support δ) (hS : ∀ y : TSet δ, y ∈' x → S.Supports y) :
+    InternallyWellOrdered hβ hγ hδ x := by
+  obtain (hx | hx) := Set.subsingleton_or_nontrivial {y : TSet δ | y ∈' x}
+  · exact Or.inl hx
+  · exact internallyWellOrdered_of_common_support_of_nontrivial hβ hγ hδ hx S hS
+
+theorem powerset_internallyWellOrdered {x : TSet δ} (h : InternallyWellOrdered hγ hδ hε x) :
+    InternallyWellOrdered hβ hγ hδ (powerset hδ hε x) := by
+  obtain ⟨S, hS⟩ := exists_common_support_of_internallyWellOrdered hγ hδ hε h
+  apply internallyWellOrdered_of_common_support hβ hγ hδ S
+  intro y hy
+  simp only [mem_powerset_iff] at hy
+  refine ⟨?_, λ h ↦ by cases h⟩
+  intro ρ hρ
+  apply ext hε
+  intro z
+  constructor
+  · intro hz
+    simp only [mem_smul_iff', allPerm_inv_sderiv'] at hz
+    have := (hS _ (hy _ hz)).supports ρ hρ
+    simp only [smul_singleton, smul_inv_smul, singleton_inj] at this
+    rwa [this]
+  · intro hz
+    have := (hS z (hy _ hz)).supports ρ hρ
+    simp only [smul_singleton, singleton_inj] at this
+    rw [← this]
+    simp only [mem_smul_iff', allPerm_inv_sderiv', inv_smul_smul]
+    exact hz
 
 end ConNF
